src/Init/Data/Array/Basic.lean
@@ -59,6 +59,8 @@ def uget (a : @& Array α) (i : USize) (h : i.toNat < a.size) : α :=
 
 instance : GetElem (Array α) USize α fun xs i => i.toNat < xs.size where
   getElem xs i h := xs.uget i h
+  getElem? xs i  := if h : i.toNat < xs.size then some (xs.uget i h) else none
+  getElem! xs i  := if h : i.toNat < xs.size then xs.uget i h else outOfBounds
 
 instance : LawfulGetElem (Array α) USize α fun xs i => i.toNat < xs.size where
 
