src/Init/Data/ByteArray/Basic.lean
@@ -51,11 +51,15 @@ def get : (a : @& ByteArray) → (@& Fin a.size) → UInt8
 
 instance : GetElem ByteArray Nat UInt8 fun xs i => i < xs.size where
   getElem xs i h := xs.get ⟨i, h⟩
+  getElem? xs i := if h : i < xs.size then some (xs.get ⟨i, h⟩) else none
+  getElem! xs i := if h : i < xs.size then xs.get ⟨i, h⟩ else outOfBounds
 
 instance : LawfulGetElem ByteArray Nat UInt8 fun xs i => i < xs.size where
 
 instance : GetElem ByteArray USize UInt8 fun xs i => i.val < xs.size where
   getElem xs i h := xs.uget i h
+  getElem? xs i := if h : i.val < xs.size then some (xs.uget i h) else none
+  getElem! xs i := if h : i.val < xs.size then xs.uget i h else outOfBounds
 
 instance : LawfulGetElem ByteArray USize UInt8 fun xs i => i.val < xs.size where
 
